Examples/UniswapV2Pair/TransferRoutines.lean
@@ -1,4 +1,5 @@
 import Examples.UniswapV2Pair.Routines
+import Examples.UniswapV2Pair.LegacyABI
 
 open Solm ABI Ethereum Ethereum.EVM Reasoning.Theory Reasoning.Reach
 
